src/program_proof/tulip/program/txn/txn_attach.v
@@ -1,0 +1,56 @@
+From Perennial.program_proof.tulip.program Require Import prelude.
+From Perennial.program_proof.tulip.program.txn Require Import txn_repr.
+From Perennial.program_proof.tulip.program.gcoord Require Import
+  gcoord_repr gcoord_attach.
+
+Section program.
+  Context `{!heapGS Σ, !tulip_ghostG Σ}.
+
+  Theorem wp_Txn__attach (txn : loc) ts γ :
+    {{{ ([∗ set] gid ∈ gids_all, own_txn_client_token γ ts gid) ∗ own_txn_init txn ts γ }}}
+      Txn__attach #txn
+    {{{ RET #(); own_txn_init txn ts γ }}}.
+  Proof.
+    iIntros (Φ) "[Hctks Htxn] HΦ".
+    wp_rec.
+
+    (*@ func (txn *Txn) attach() {                                              @*)
+    (*@     for _, gcoord := range(txn.gcoords) {                               @*)
+    (*@         gcoord.Attach(txn.ts)                                           @*)
+    (*@     }                                                                   @*)
+    (*@ }                                                                       @*)
+    do 2 iNamed "Htxn". iNamed "Hgcoords".
+    wp_loadField.
+    set P := (λ (mx : gmap u64 loc),
+                "Hts"   ∷ own_txn_ts txn ts ∗
+                "Hctks" ∷ [∗ set] gid ∈ gids_all ∖ (dom mx), own_txn_client_token γ ts gid)%I.
+    wp_apply (wp_MapIter_fold _ _ _ P with "Hgcoords [$Hts Hctks]").
+    { subst P. simpl. by rewrite dom_empty_L difference_empty_L. }
+    { clear Φ.
+      iIntros (m g p Φ) "!> [HP %Hp] HΦ".
+      destruct Hp as [Hnotin Hin].
+      iNamed "HP". iNamed "Hts".
+      wp_loadField.
+      iDestruct (big_sepS_delete _ _ g with "Hctks") as "[Hctk Hctks]".
+      { apply not_elem_of_dom_2 in Hnotin.
+        apply elem_of_dom_2 in Hin.
+        set_solver.
+      }
+      iDestruct (big_sepM_lookup with "Hgcoordsabs") as "Hgcoordabs".
+      { apply Hin. }
+      wp_apply (wp_GroupCoordinator__Attach with "Hgcoordabs [Hctk]").
+      { by rewrite Htsword. }
+      iApply "HΦ".
+      iFrame "∗ %".
+      by rewrite dom_insert_L difference_difference_l_L union_comm_L.
+    }
+    iIntros "[Hgcoords HP]".
+    iNamed "HP".
+    wp_pures.
+    iApply "HΦ".
+    iAssert (own_txn_gcoords txn γ)%I with "[Hgcoords HgcoordsP]" as "Hgcoords".
+    { by iFrame "∗ # %". }
+    by iFrame "∗ # %".
+  Qed.
+
+End program.
